Determinisim Proofs

IRNodeHierarchy.thy
@@ -218,6 +218,7 @@ fun is_sequential_node :: "IRNode \<Rightarrow> bool" where
   "is_sequential_node (LoopBeginNode _ _ _ _) = True" |
   "is_sequential_node (LoopExitNode _ _ _) = True" |
   "is_sequential_node (SignedDivNode _ _ _ _ _) = True" |
-  "is_sequential_node n = isAbstractMergeNodeType n"
+  "is_sequential_node (MergeNode _ _ _) = True" |
+  "is_sequential_node _ = False"
 
 end
